WIP, after meeting

src/Vellvm/genericvalues_inject.v
@@ -27,8 +27,10 @@ Import LLVMtypings.
    injection. *)
 Inductive gv_inject (mi: meminj) : GenericValue -> GenericValue -> Prop :=
 | gv_inject_nil : gv_inject mi nil nil
-| gv_inject_cons : forall v1 m v2 gv1 gv2, 
-    MoreMem.val_inject mi v1 v2 -> gv_inject mi gv1 gv2 -> 
+| gv_inject_cons : forall
+    v1 m v2 gv1 gv2
+    (CHUNK: v1 = Vundef -> v2 <> Vundef -> Val.has_chunkb v2 m),
+    MoreMem.val_inject mi v1 v2 -> gv_inject mi gv1 gv2 ->
     gv_inject mi ((v1,m)::gv1) ((v2,m)::gv2)
 .
 
@@ -129,20 +131,51 @@ Proof.
   induction mcs; simpl; auto.
 Qed.
 
+Lemma gv_inject_mc2undefs': forall mi mcs gvs',
+  gv_chunks_match_typb_aux gvs' mcs = true ->
+  gv_inject mi (mc2undefs mcs) gvs'.
+Proof.
+  unfold mc2undefs.
+  induction mcs; ii; ss.
+  - destruct gvs'; ss. des_ifs.
+  - destruct gvs'; ss. des_ifs.
+    apply andb_true_iff in H. des.
+    apply andb_true_iff in H. des.
+    apply memory_chunk_eq_prop in H. subst.
+    econs; eauto.
+Qed.
+
 Lemma gv_inject_gundef : forall mi TD t gv, gundef TD t = Some gv -> gv_inject mi gv gv.
 Proof.
   intros. unfold gundef in H. 
   inv_mbind. apply gv_inject_mc2undefs.
 Qed.
 
+Lemma gv_inject_gundef'
+      mi TD t gv gv'
+      (MATCH: gv_chunks_match_typb TD gv' t = true)
+      (UNDEF: gundef TD t = Some gv)
+  :
+    gv_inject mi gv gv'
+.
+Proof.
+  intros. unfold gundef in UNDEF. 
+  inv_mbind. (* apply gv_inject_mc2undefs. *)
+  unfold gv_chunks_match_typb in *. des_ifs.
+  eapply gv_inject_mc2undefs'; eauto.
+Qed.
+
+Ltac chunk_simpl := i; clarify.
+Ltac chunk_auto := econs; eauto; chunk_simpl.
+Ltac chunk_auto_try := try (by chunk_auto).
+
 Lemma gv_inject_nptr_val_refl : forall TD v mi m,
   (forall b ofs, v <> Vptr b ofs) ->
   gv_inject mi (val2GV TD v m) (val2GV TD v m).
 Proof.
   intros. unfold val2GV.
-  destruct v; auto.
-    
-    assert (J:=@H b i0). contradict J; auto.
+  destruct v; chunk_auto.
+  - assert (J:=@H b i0). contradict J; auto.
 Qed.
 
 Lemma gv_inject__same_size : forall mi gv1 gv2,
@@ -159,6 +192,34 @@ Proof.
   induction 1; intros; simpl; auto.
 Qed.
 
+Require Import Classical.
+
+(* TODO: move to memory_sim.v *)
+Lemma val_inject__has_chunkb: forall mi v1 v2 m
+  (H : MoreMem.val_inject mi v1 v2)
+  (CHUNK: v1 = Vundef -> v2 <> Vundef -> Val.has_chunkb v2 m)
+  ,
+  Val.has_chunkb v1 m = Val.has_chunkb v2 m.
+Proof.
+  intros. inv H; auto.
+  destruct (classic (v2 = Vundef)).
+  - subst. ss.
+  - exploit CHUNK; eauto.
+Qed.
+
+Lemma gv_inject__has_chunkb: forall mi gv1 gv2
+  (H: gv_inject mi gv1 gv2),
+  List.Forall2 (fun vm1 vm2 =>
+                  Val.has_chunkb vm1.(fst) vm1.(snd) =
+                  Val.has_chunkb vm2.(fst) vm2.(snd)) gv1 gv2
+.
+Proof.
+  ii. ginduction H; ii; ss.
+  econs; eauto.
+  s.
+  eapply val_inject__has_chunkb; eauto.
+Qed.
+
 Lemma simulation__gv_chunks_match_typb : forall mi TD gv gv' t,
   gv_inject mi gv gv' ->
   gv_chunks_match_typb TD gv t = gv_chunks_match_typb TD gv' t.
@@ -169,8 +230,8 @@ Proof.
   generalize dependent l0.
   induction H; simpl; auto.
     destruct l0; auto.
-    apply MoreMem.val_inject__has_chunkb with (m:=m) in H; auto.
-      congruence.
+    rewrite IHgv_inject; try eassumption. f_equal. f_equal.
+    eapply val_inject__has_chunkb; eauto.
 Qed.
 
 (* Globals inject to themselves. *)
@@ -182,13 +243,14 @@ Proof.
   induction gv; intros; simpl; auto.
     destruct a.
     destruct v; simpl in *; try solve 
-        [assert (J:=@IHgv H H0); eauto].
+        [assert (J:=@IHgv H H0); eauto]; chunk_auto_try.
 
         destruct H0 as [H1 H2].
         assert (J:=(@IHgv H H2)).
         inversion H.
         apply mi_globals0 in H1.
         apply gv_inject_cons; auto.
+          { chunk_simpl. }
           apply MoreMem.val_inject_ptr with (delta:=0); auto.
             rewrite Int.add_zero; auto.
 Qed.
@@ -719,12 +781,22 @@ Proof.
     simpl. rewrite J1.
     remember (splitGenericValue gvr (Z_of_nat n)) as R1.
     destruct R1 as [[gvrl gvrr]|]; inv H2.
+    {
       symmetry in HeqR1.
       eapply simulation__splitGenericValue_some in HeqR1; eauto.      
       destruct HeqR1 as [gvrl' [gvrr' [J1' [J2' J3']]]].
-      simpl. rewrite J1'. 
-      erewrite <- simulation__gv_chunks_match_typb; eauto.
-      destruct_if; eauto using gv_inject_gundef.
+      simpl. rewrite J1'.
+        erewrite <- simulation__gv_chunks_match_typb; eauto.
+        destruct_if; eauto using gv_inject_gundef.
+        (* des_ifs; try (by esplits; eauto using gv_inject_gundef'). *)
+        (* - rename gv into __gv__. *)
+        (*   unfold gv_chunks_match_typb in *. unfold gundef. des_ifs. *)
+        (*   esplits; eauto. *)
+        (*   admit. *)
+        (* - unfold gundef in *. unfold gv_chunks_match_typb in *. des_ifs. *)
+        (*   esplits; eauto. *)
+        (*   apply gv_inject_mc2undefs. *)
+    }
 
       symmetry in HeqR1.
       eapply simulation__splitGenericValue_none in HeqR1; eauto.      
@@ -736,629 +808,37 @@ Proof.
     rewrite HeqR. rewrite H2. eauto using gv_inject_gundef.
 Qed.
 
-Lemma simulation__insertGenericValue: forall mi gv1 gv1' TD t1 l0 gv t2 gv2 gv2',
-  gv_inject mi gv1 gv1' ->
-  gv_inject mi gv2 gv2' ->
-  insertGenericValue TD t1 gv1 l0 t2 gv2 = Some gv ->
-  exists gv',
-    insertGenericValue TD t1 gv1' l0 t2 gv2' = Some gv' /\
-    gv_inject mi gv gv'.
+(* TODO: location *)
+Lemma has_chunk__has_chunkb
+      v chk 
+      (CHUNK: Val.has_chunk v chk)
+  :
+    <<CHUNK: Val.has_chunkb v chk = true>>
+.
 Proof.
-  intros mi gv1 gv1' TD t1 l0 gv t2 gv2 gv2' H H0 H1.
-  unfold insertGenericValue in *.
-  destruct (intConsts2Nats TD l0); inv H1; eauto using gv_inject_gundef.
-  destruct (mgetoffset TD t1 l1) as [[o ?]|]; inv H3; eauto using gv_inject_gundef.
-  unfold mset in *. 
-  destruct (getTypeStoreSize TD t2); inv H2; eauto using gv_inject_gundef.
-  assert (J:=@gv_inject_length_eq mi gv2 gv2' H0). 
-  rewrite <- J. simpl.
-  destruct (n =n= length gv2); subst; inv H3; eauto using gv_inject_gundef.
-  remember (splitGenericValue gv1 o) as R.
-  destruct R as [[gvl gvr]|].
-    symmetry in HeqR.
-    eapply simulation__splitGenericValue_some in HeqR; eauto.      
-    destruct HeqR as [gvl' [gvr' [J1 [J2 J3]]]].
-    simpl. rewrite J1.
-    remember (splitGenericValue gvr (Z_of_nat n)) as R1.
-    destruct R1 as [[gvrl gvrr]|]; inv H2.
-      symmetry in HeqR1.
-      eapply simulation__splitGenericValue_some in HeqR1; eauto.      
-      destruct HeqR1 as [gvrl' [gvrr' [J1' [J2' J3']]]].
-      simpl. rewrite J1'. 
-      erewrite <- simulation__gv_chunks_match_typb; eauto.
-      destruct_if; eauto using gv_inject_gundef.
-      exists (gvl' ++ gv2' ++ gvrr').
-      split; auto.
-        apply gv_inject_app; auto.
-        apply gv_inject_app; auto.
-
-      symmetry in HeqR1.
-      eapply simulation__splitGenericValue_none in HeqR1; eauto.      
-      rewrite HeqR1. eauto using gv_inject_gundef.
-    symmetry in HeqR.
-    eapply simulation__splitGenericValue_none in HeqR; eauto.      
-    rewrite HeqR. rewrite H2. eauto using gv_inject_gundef.
-Qed.
-
-Lemma simulation__mtrunc_refl : forall mi TD top t1 gv1 t2 gv2,
-  gv_inject mi gv1 gv1 ->
-  mtrunc TD top t1 t2 gv1 = Some gv2 ->
-  gv_inject mi gv2 gv2.
-Proof.
-  intros.
-  apply gv_inject__val_inject with (TD:=TD) in H.
-  destruct H as [v1 [v2 [J1 [J2 J3]]]].
-  unfold mtrunc in *.
-  rewrite J1 in H0. 
-  rewrite J1 in J2. inv J2.
-  destruct v2; try (inv J3); try solve [inv H0; eauto using gv_inject_gundef].
-    destruct_typ t1; try solve [
-      inv H0; eauto using gv_inject_gundef |
-      destruct_typ t2; try solve 
-        [inv H0; eauto using gv_inject_gundef | 
-         inv H0; destruct (le_lt_dec wz (s1-1)); unfold val2GV; simpl; auto]
-    ].
-
-    destruct_typ t1; try solve [
-      inv H0; eauto using gv_inject_gundef |
-      destruct_typ t2; try solve [
-        inv H0; eauto using gv_inject_gundef |
-        match goal with
-        | H: context [floating_point_order ?f1 ?f0] |- _ =>
-          destruct (floating_point_order f1 f0); try solve [
-            destruct f0; try solve 
-              [inv H0; unfold val2GV; simpl; eauto using gv_inject_gundef] |
-            inv H0; eauto using gv_inject_gundef
-          ]
-        end
-      ]
-    ].
-
-    destruct_typ t1; try solve [
-      inv H0; eauto using gv_inject_gundef |
-      destruct_typ t2; try solve [
-        inv H0; eauto using gv_inject_gundef |
-        match goal with
-        | H: context [floating_point_order ?f1 ?f0] |- _ =>
-          destruct (floating_point_order f1 f0); try solve [
-            destruct f0; try solve 
-              [inv H0; unfold val2GV; simpl; eauto using gv_inject_gundef] |
-            inv H0; eauto using gv_inject_gundef
-          ]
-        end
-      ]
-    ].
-Qed.
-
-Lemma simulation__mext_refl : forall mi TD eop t1 gv1 t2 gv2,
-  gv_inject mi gv1 gv1 ->
-  mext TD eop t1 t2 gv1 = Some gv2 ->
-  gv_inject mi gv2 gv2.
-Proof.
-  intros. assert (J0:=H).
-  apply gv_inject__val_inject with (TD:=TD) in H.
-  destruct H as [v1 [v2 [J1 [J2 J3]]]].
-  unfold mext in *.
-  rewrite J1 in H0.
-  rewrite J1 in J2. inv J2.
-  destruct t1; destruct t2; inv H0; eauto using gv_inject_gundef.
-    destruct v2; inv H1; eauto using gv_inject_gundef.
-    destruct eop; inv H0; try solve [
-      eauto using gv_inject_gundef | unfold val2GV; simpl; auto].
-    match goal with
-    | H: context [floating_point_order ?f ?f0] |- _ =>
-      destruct (floating_point_order f f0); inv H1; try solve [
-        eauto using gv_inject_gundef | unfold val2GV; simpl; auto]
-    end.
-    destruct v2; inv H0; eauto using gv_inject_gundef.
-    destruct eop; inv H1; eauto using gv_inject_gundef.
-    match goal with
-      | f : floating_point, H : ?t = ret _ |- _ =>
-        match t with
-          | context[f] =>
-            destruct f; inv H0; unfold val2GV; auto            
-        end
-    end.
-Qed.
-
-Lemma simulation__mbop_refl : forall mi TD op bsz gv1 gv2 gv3,
-  gv_inject mi gv1 gv1 ->
-  gv_inject mi gv2 gv2 ->
-  mbop TD op bsz gv1 gv2 = Some gv3 ->
-  gv_inject mi gv3 gv3.
-Proof.
-  intros. assert (J0:=H0). assert (J:=H).
-  apply gv_inject__val_inject with (TD:=TD) in H.
-  destruct H as [v1 [v1' [J1 [J2 J3]]]].
-  apply gv_inject__val_inject with (TD:=TD) in H0.
-  destruct H0 as [v2 [v2' [J1' [J2' J3']]]].
-  rewrite J1 in J2. inv J2.
-  rewrite J1' in J2'. inv J2'.
-  unfold mbop in *.
-  rewrite J1 in H1. rewrite J1' in H1. 
-  destruct v1';
-    try solve [inv H1; eauto using gv_inject_gundef].
-  destruct v2';
-    try solve [inv H1; eauto using gv_inject_gundef].
-  destruct (eq_nat_dec (wz + 1) (Size.to_nat bsz)); 
-     try solve [inv H1; eauto using gv_inject_gundef].
-  destruct op;
-  try match goal with
-      | H0 : match ?s with
-        | ret _ => _
-        | merror => _
-        end = _ |- _ => destruct s eqn:Heqn
-  end;
-  inv H1; try (apply gv_inject_nptr_val_refl; auto); eauto using gv_inject_gundef.
-       apply add_isnt_ptr.
-       apply sub_isnt_ptr.
-       apply mul_isnt_ptr.
-       intros; eapply divu_isnt_ptr; eauto.
-       intros; eapply divs_isnt_ptr; eauto.
-       intros; eapply modu_isnt_ptr; eauto.
-       intros; eapply mods_isnt_ptr; eauto.
-       apply shl_isnt_ptr.
-       intros; eapply shrx_isnt_ptr; eauto.
-       apply shr_isnt_ptr.
-       apply and_isnt_ptr.
-       apply or_isnt_ptr.
-       apply xor_isnt_ptr.
-Qed.
-
-Lemma simulation__mfbop_refl : forall mi TD op fp gv1 gv2 gv3,
-  gv_inject mi gv1 gv1 ->
-  gv_inject mi gv2 gv2 ->
-  mfbop TD op fp gv1 gv2 = Some gv3 ->
-  gv_inject mi gv3 gv3.
-Proof.
-  intros. assert (J0:=H0). assert (J:=H).
-  apply gv_inject__val_inject with (TD:=TD) in H.
-  destruct H as [v1 [v1' [J1 [J2 J3]]]].
-  apply gv_inject__val_inject with (TD:=TD) in H0.
-  destruct H0 as [v2 [v2' [J1' [J2' J3']]]].
-  rewrite J1 in J2. inv J2.
-  rewrite J1' in J2'. inv J2'.
-  unfold mfbop in *.
-  rewrite J1 in H1. rewrite J1' in H1. 
-  destruct v1';
-    try solve [inv H1; eauto using gv_inject_gundef];
-  destruct v2';
-    try solve [inv H1; eauto using gv_inject_gundef];
-  destruct fp; try solve [inv H1; eauto using gv_inject_gundef];
-  destruct op; inv H1; 
-    try (apply gv_inject_nptr_val_refl; try solve [auto | intro; congruence]).
-Qed.
-
-Lemma simulation__mcast_refl : forall mi TD op t1 t2 gv1 gv2,
-  gv_inject mi gv1 gv1 ->
-  mcast TD op t1 t2 gv1 = Some gv2 ->
-  gv_inject mi gv2 gv2.
-Proof.
-  intros.  assert (J:=H).
-  apply gv_inject__val_inject with (TD:=TD) in H.
-  destruct H as [v1 [v1' [J1 [J2 J3]]]].
-  rewrite J1 in J2. inv J2.
-  unfold mcast, mbitcast in *.
-  destruct op; 
-    try solve [
-      inv H0; eauto using gv_inject_gundef |
-      destruct t1; destruct t2; inv H0; eauto using gv_inject_gundef
-    ].
-Qed.
-
-Lemma simulation__micmp_refl : forall mi TD c t gv1 gv2 gv3,
-  gv_inject mi gv1 gv1 ->
-  gv_inject mi gv2 gv2 ->
-  micmp TD c t gv1 gv2 = Some gv3 ->
-  gv_inject mi gv3 gv3.
-Proof.
-  intros. assert (J0:=H0). assert (J:=H).
-  apply gv_inject__val_inject with (TD:=TD) in H.
-  destruct H as [v1 [v1' [J1 [J2 J3]]]].
-  apply gv_inject__val_inject with (TD:=TD) in H0.
-  destruct H0 as [v2 [v2' [J1' [J2' J3']]]].
-  rewrite J1 in J2. inv J2.
-  rewrite J1' in J2'. inv J2'.
-  unfold micmp, micmp_int in *.
-  rewrite J1 in H1. rewrite J1' in H1. 
-  destruct t; try solve [inv H1; eauto using gv_inject_gundef].
-  destruct v1'; try solve [inv H1; eauto using gv_inject_gundef].
-  destruct v2'; try solve [inv H1; eauto using gv_inject_gundef].
-  destruct c; inv H1; 
-        try (apply gv_inject_nptr_val_refl; try solve 
-            [auto | apply cmp_isnt_ptr | apply cmpu_isnt_ptr
-            | apply cmpu_int_isnt_ptr]).
-Qed.
-
-Lemma simulation__mfcmp_refl : forall mi TD c t gv1 gv2 gv3,
-  gv_inject mi gv1 gv1 ->
-  gv_inject mi gv2 gv2 ->
-  mfcmp TD c t gv1 gv2 = Some gv3 ->
-  gv_inject mi gv3 gv3.
-Proof.
-  intros. assert (J0:=H0). assert (J:=H).
-  apply gv_inject__val_inject with (TD:=TD) in H.
-  destruct H as [v1 [v1' [J1 [J2 J3]]]].
-  apply gv_inject__val_inject with (TD:=TD) in H0.
-  destruct H0 as [v2 [v2' [J1' [J2' J3']]]].
-  rewrite J1 in J2. inv J2.
-  rewrite J1' in J2'. inv J2'.
-  unfold mfcmp in *.
-  rewrite J1 in H1. rewrite J1' in H1. 
-  destruct v1'; try solve [inv H1; eauto using gv_inject_gundef].
-  destruct v2'; try solve [inv H1; eauto using gv_inject_gundef].
-  destruct t; try solve [inv H1; eauto using gv_inject_gundef].
-  destruct c; inv H1; try (
-    apply gv_inject_nptr_val_refl; try solve 
-            [auto | apply val_of_bool_isnt_ptr | apply Vfalse_isnt_ptr | 
-             apply Vtrue_isnt_ptr]
-    ).
-    eauto using gv_inject_gundef.
-    eauto using gv_inject_gundef.
-  destruct c; inv H1; try (
-    apply gv_inject_nptr_val_refl; try solve 
-            [auto | apply val_of_bool_isnt_ptr | apply Vfalse_isnt_ptr | 
-             apply Vtrue_isnt_ptr]
-    ).
-Qed.
-
-Lemma simulation__mgep_refl : forall mi TD v v0 t0 l1,
-  MoreMem.val_inject mi v v ->
-  mgep TD t0 v l1 = Some v0 ->
-  MoreMem.val_inject mi v0 v0.
-Proof.
-  intros.
-  unfold mgep in *.
-  destruct v; tinv H0.
-  destruct l1; tinv H0.
-  destruct (mgetoffset TD (typ_array 0%nat t0) (z :: l1)) as [[o ?]|]; tinv H0.
-  inv H0.
-  inversion H. subst i0 b ofs1 b1.
-  eapply MoreMem.val_inject_ptr; eauto.
-    assert (Int.add 31 ofs2 (Int.repr 31 delta) = 
-            Int.add 31 (Int.repr 31 delta) ofs2) as EQ.
-      rewrite <- Int.add_commut. auto. 
-    symmetry.
-    rewrite Int.add_commut. 
-    rewrite <- Int.add_assoc.
-    rewrite <- EQ.   
-    rewrite <- H5.
-    auto.
-Qed.
-
-Lemma GV2ptr_refl : forall mi TD gv v,
-  gv_inject mi gv gv ->
-  GV2ptr TD (getPointerSize TD) gv = Some v ->
-  MoreMem.val_inject mi v v.
-Proof.
-  intros.
-  unfold GV2ptr in H0.
-  destruct gv; tinv H0.
-  destruct p; tinv H0.
-  destruct v0; tinv H0.
-  destruct gv; tinv H0.
-  inv H0. inv H; auto.
-Qed.
-
-Lemma simulation__splitGenericValue_refl : forall mi gv z gvl gvr,
-  gv_inject mi gv gv ->
-  splitGenericValue gv z = Some (gvl, gvr) ->
-  gv_inject mi gvl gvl /\
-  gv_inject mi gvr gvr.
-Proof.
-  induction gv; simpl; intros; inv H; simpl.
-    destruct (zeq z 0); inv H0. 
-      auto.
-      destruct (zlt z 0); inv H1.
-
-    destruct (zeq z 0); inv H0. 
-      split; auto.
-
-      destruct (zlt z 0); inv H1.
-      remember (splitGenericValue gv (z - size_chunk m)) as R.
-      destruct R as [[gvl' gvr']|]; inv H0.
-      symmetry in HeqR. 
-      eapply IHgv in HeqR; eauto.
-      destruct HeqR as [J5 J6].
-      split; auto.
-Qed.
-
-Lemma simulation__extractGenericValue_refl : forall mi gv1 TD t1 l0 gv,
-  gv_inject mi gv1 gv1 ->
-  extractGenericValue TD t1 gv1 l0 = Some gv ->
-  gv_inject mi gv gv.
-Proof.
-  intros.
-  unfold extractGenericValue in *.
-  destruct (intConsts2Nats TD l0); inv H0;
-    try solve [auto using gv_inject_uninits].
-  destruct (mgetoffset TD t1 l1) as [[o t']|]; inv H2;
-    try solve [auto using gv_inject_uninits].
-  unfold mget in *. 
-  destruct (getTypeStoreSize TD t'); inv H1; 
-    try solve [eauto using gv_inject_gundef].
-  remember (splitGenericValue gv1 o) as R.
-  destruct R as [[gvl gvr]|]; inv H2;
-    try solve [eauto using gv_inject_gundef].
-  symmetry in HeqR.
-  eapply simulation__splitGenericValue_refl in HeqR; eauto.      
-  destruct HeqR as [J2 J3].
-  remember (splitGenericValue gvr (Z_of_nat n)) as R1.
-  destruct R1 as [[gvrl gvrr]|]; inv H1;
-    try solve [eauto using gv_inject_gundef].
-  symmetry in HeqR1.
-  eapply simulation__splitGenericValue_refl in HeqR1; eauto.      
-  destruct HeqR1; auto.
-  destruct_if; eauto using gv_inject_gundef.
-Qed.
-
-Lemma simulation__insertGenericValue_refl : forall mi gv1 TD t1 l0 gv t2 gv2,
-  gv_inject mi gv1 gv1 ->
-  gv_inject mi gv2 gv2 ->
-  insertGenericValue TD t1 gv1 l0 t2 gv2 = Some gv ->
-  gv_inject mi gv gv.
-Proof.
-  intros.
-  unfold insertGenericValue in *.
-  destruct (intConsts2Nats TD l0); inv H1; 
-    try solve [eauto using gv_inject_gundef].
-  destruct (mgetoffset TD t1 l1) as [[o ?]|]; inv H3;
-    try solve [eauto using gv_inject_gundef].
-  unfold mset in *. 
-  destruct (getTypeStoreSize TD t2); inv H2; 
-    try solve [eauto using gv_inject_gundef].
-  destruct (n =n= length gv2); subst;
-    try solve [inv H3; eauto using gv_inject_gundef].
-  remember (splitGenericValue gv1 o) as R.
-  destruct R as [[gvl gvr]|]; inv H3;
-    try solve [eauto using gv_inject_gundef].
-  symmetry in HeqR.
-  eapply simulation__splitGenericValue_refl in HeqR; eauto.      
-  destruct HeqR as [J2 J3].
-  remember (splitGenericValue gvr (Z_of_nat n)) as R1.
-  destruct R1 as [[gvrl gvrr]|]; inv H2;
-    try solve [eauto using gv_inject_gundef].
-  symmetry in HeqR1.
-  eapply simulation__splitGenericValue_refl in HeqR1; eauto.      
-  destruct HeqR1.
-  destruct_if; eauto using gv_inject_gundef.
-  apply gv_inject_app; auto.
-  apply gv_inject_app; auto.
-Qed.
-
-Lemma simulation__eq__GV2int : forall mi gn gn' TD sz,
-  gv_inject mi gn gn' ->
-  GV2int TD sz gn = GV2int TD sz gn'.
-Proof.
-(*   intros mi gn gn' TD sz Hinj. *)
-(*   unfold GV2int. *)
-(*   destruct gn. *)
-(*     inv Hinj. subst. auto. *)
-
-(*     inv Hinj. *)
-(*     inv H1; auto. *)
-(*     destruct gn; inv H3; auto. *)
-(* Qed. *)
-Admitted.
-
-Lemma simulation__GVs2Nats : forall mi TD vidxs vidxs',
-  gvs_inject mi vidxs vidxs' ->
-  GVs2Nats TD vidxs = GVs2Nats TD vidxs'.
-Proof.
-  induction vidxs; intros vidxs' Hinj.
-    destruct vidxs'; inv Hinj; simpl; auto.
-    destruct vidxs'; simpl in *; inv Hinj; auto.
-      erewrite simulation__eq__GV2int; eauto.      
-      erewrite IHvidxs; eauto.
-Qed.
-
-Lemma simulation__mgep' : forall mi TD v v' t0 l1,
-  MoreMem.val_inject mi v v' ->
-  mgep TD t0 v l1 = None -> 
-  mgep TD t0 v' l1 = None.
-Proof.
-(*   intros. *)
-(*   unfold mgep in *. *)
-(*   inv H; auto. *)
-(*   destruct l1; auto. *)
-(*   destruct (mgetoffset TD (typ_array 0%nat t0) (z :: l1)) as [[i1 ?]|];  *)
-(*     try solve [inv H0 | auto]. *)
-(* Qed. *)
-Admitted.
-
-Lemma simulation__GV2ptr' : forall mi TD gv1 gv1',
-  gv_inject mi gv1 gv1' ->
-  GV2ptr TD (getPointerSize TD) gv1 = None ->
-  GV2ptr TD (getPointerSize TD) gv1' = None.
-Proof.
-(*   intros. *)
-(*   unfold GV2ptr in *. *)
-(*   destruct gv1'; auto. *)
-(*   destruct p. *)
-(*   destruct v; auto. *)
-(*   destruct gv1'; auto. *)
-(*   destruct gv1; tinv H. *)
-(*   destruct p; tinv H. *)
-(*   inv H. inv H8. inv H3; tinv H0. *)
-(* Qed. *)
-Admitted.
-
-Lemma simulation__GEP : forall maxb mi TD Mem Mem2 inbounds0 vidxs vidxs' gvp1 
-    gvp gvp' t t',
-  wf_sb_mi maxb mi Mem Mem2 ->
-  gv_inject mi gvp gvp' ->
-  gvs_inject mi vidxs vidxs' ->
-  GEP TD t gvp vidxs inbounds0 t' = ret gvp1 ->
-  exists gvp2,
-    GEP TD t gvp' vidxs' inbounds0 t' = ret gvp2 /\
-    gv_inject mi gvp1 gvp2.
-Proof.
-  intros maxb mi TD Mem Mem2 inbounds0 vidxs vidxs' gvp1 gvp gvp' t t' H H0 H1 
-    H2.
-  unfold GEP in *.
-  remember (GV2ptr TD (getPointerSize TD) gvp) as R.
-  destruct R; inv H2.
-    symmetry in HeqR.
-    eapply simulation__GV2ptr in HeqR; eauto.
-    destruct HeqR as [v' [J1 J2]].
-    rewrite J1. 
-    assert (GVs2Nats TD vidxs = GVs2Nats TD vidxs') as EQ.
-      eapply simulation__GVs2Nats; eauto.
-    rewrite <- EQ.
-    destruct (GVs2Nats TD vidxs).
-      remember (mgep TD t v l0) as R1.
-      destruct R1; inv H4.
-        symmetry in HeqR1.
-        eapply simulation__mgep in HeqR1; eauto.
-        destruct HeqR1 as [v0' [J11 J12]].
-        rewrite J11. exists (ptr2GV TD v0').
-        unfold ptr2GV, val2GV.
-        simpl. eauto.
-
-        symmetry in HeqR1.
-        eapply simulation__mgep' in HeqR1; eauto.
-        rewrite HeqR1. simpl. 
-        unfold gundef. simpl.
-        eauto using gv_inject_gundef.
-
-      rewrite H4. eauto using gv_inject_gundef.
-
-    erewrite simulation__GV2ptr'; eauto.
-    unfold gundef. simpl.
-    eauto using gv_inject_gundef.
-Qed.
-
-(* The sb_ds_trans_lib.mem_simulation__free should use this lemma. *)
-Lemma mem_inj__free : forall mi Mem0 M2 Mem' mgb hi lo
-  (b2 : Values.block) (delta : Z) blk,
-  wf_sb_mi mgb mi Mem0 M2 ->
-  MoreMem.mem_inj mi Mem0 M2 ->
-  Mem.free Mem0 blk lo hi = ret Mem' ->
-  (lo, hi) = Mem.bounds Mem0 blk ->
-  mi blk = ret (b2, delta) ->
-  exists Mem2',
-    Mem.free M2 b2 (lo+delta) (hi+delta) = ret Mem2' /\
-    wf_sb_mi mgb mi Mem' Mem2' /\
-    MoreMem.mem_inj mi Mem' Mem2'.
-Proof.
-  intros mi Mem0 M2 Mem' mgb hi lo b2 delta blk Hwfmi Hmsim1 H0 HeqR2 H4.
-  assert ({ Mem2':Mem.mem | Mem.free M2 b2 (lo+delta) (hi+delta) = ret Mem2'})
-    as J.
-    apply Mem.range_perm_free.
-    apply Mem.free_range_perm in H0.
-    clear - H0 Hmsim1 H4.
-    unfold Mem.range_perm in *.
-    intros ofs J.
-    assert (lo <= ofs - delta < hi) as J'.
-      auto with zarith.
-    apply H0 in J'.
-    eapply MoreMem.perm_inj in J'; eauto.
-    assert (ofs - delta + delta = ofs) as EQ. auto with zarith.
-    rewrite EQ in J'. auto.
-  destruct J as [Mem2' J].
-  exists Mem2'. split; auto.
+  unfold Val.has_chunk in *.
+  destruct v, chk; simpl; intros; try solve [auto | congruence];
+    des; clarify.
+  apply andb_true_iff.
   split.
-  SCase "wfmi".
-    clear - Hwfmi H0 J H4.
-    inversion_clear Hwfmi.
-    split; eauto with mem.
-    SSCase "Hmap3".
-      intros. erewrite Mem.nextblock_free in H; eauto.
-    SSCase "Hmap4".
-      intros. erewrite Mem.nextblock_free; eauto.
-    SSCase "bounds".
-      intros. apply mi_bounds0 in H.
-      erewrite Mem.bounds_free; eauto.
-      erewrite Mem.bounds_free with (m2:=Mem2'); eauto.
-
-  SCase "msim".
-    clear - Hmsim1 Hwfmi H0 J H4.
-    inv Hwfmi.
-    eapply MoreMem.free_inj; eauto.
+  + apply andb_true_iff.
+    destruct (eq_nat_dec n n); ss. split; ss.
+    destruct (zle 0 (Int.unsigned n i0)); ss.
+  + destruct (zlt (Int.unsigned n i0) (Int.modulus n)); ss.
 Qed.
 
-(* The sb_ds_trans_lib.mem_simulation__free should use this lemma. *)
-Lemma mem_inj__unchecked_free : forall mi Mem0 M2 Mem' mgb hi lo
-  (b2 : Values.block) (delta : Z) blk,
-  wf_sb_mi mgb mi Mem0 M2 ->
-  MoreMem.mem_inj mi Mem0 M2 ->
-  Mem.unchecked_free Mem0 blk lo hi = Mem' ->
-  (lo, hi) = Mem.bounds Mem0 blk ->
-  mi blk = ret (b2, delta) ->
-  exists Mem2',
-    Mem.unchecked_free M2 b2 (lo+delta) (hi+delta) = Mem2' /\
-    wf_sb_mi mgb mi Mem' Mem2' /\
-    MoreMem.mem_inj mi Mem' Mem2'.
+(* TODO: move position *)
+Lemma load_implies_has_chunkb
+      mc Mem0 b0 ofs v0
+      (LOAD: Mem.load mc Mem0 b0 ofs = ret v0)
+  :
+  <<CHUNK: Val.has_chunkb v0 mc>>
+.
 Proof.
-  ii.
-  esplits; eauto.
-  - inv H. econs; eauto.
-  - eapply MoreMem.unchecked_free_inj; eauto.
-    + inv H; ss.
-    + inv H; ss.
-Qed.
-
-Lemma val_inject_has_chunk mi v1 v2 chk
-  (Hinj: MoreMem.val_inject mi v1 v2) :
-  has_chunk_eq v1 chk = has_chunk_eq v2 chk.
-Proof.
-(*   destruct v1, v2; inv Hinj; auto. *)
-(* Qed. *)
-Admitted.
-
-(* sb_ds_trans_lib.simulation_mstore_aux should use this *)
-Lemma mem_inj_mstore_aux : forall b b2 delta mi mgb
-  (H1 : mi b = ret (b2, delta)) mc gv ofs gv2 Mem0 Mem2 Mem0'
-  (Hwfmi : wf_sb_mi mgb mi Mem0 Mem2)
-  (Hmsim : MoreMem.mem_inj mi Mem0 Mem2)
-  (Hinj : gv_inject mi gv gv2)
-  (Hmstores : mstore_aux Mem0 mc gv b ofs = ret Mem0'),
-   exists Mem2',
-     mstore_aux Mem2 mc gv2 b2 (ofs + delta) = ret Mem2' /\
-     wf_sb_mi mgb mi Mem0' Mem2' /\
-     MoreMem.mem_inj mi Mem0' Mem2'.
-Proof.
-  induction mc; destruct gv; simpl; intros.
-    inv Hinj; inv Hmstores; eauto.
-    inv Hinj; inv Hmstores; eauto.
-    inv Hinj; inv Hmstores; eauto.
-    destruct p. inv Hinj.
-    destruct (AST.memory_chunk_eq a m); simpl in *; tinv Hmstores.
-    rewrite <- (val_inject_has_chunk mi v v2 m H4).
-    destruct (has_chunk_eq v m); simpl in *; tinv Hmstores.
-    remember (Mem.store m Mem0 b ofs v) as R1.
-    destruct R1 as [M|]; tinv Hmstores.
-    symmetry in HeqR1.
-    inv Hwfmi.
-    assert (Hmstore0 := HeqR1).
-    eapply MoreMem.store_mapped_inj with (f:=mi)(m2:=Mem2) in HeqR1;
-      try solve [eauto | inversion Hwfmi; eauto].
-    destruct HeqR1 as [Mem2' [Hmstore Hminj]].
-    simpl. rewrite Hmstore.
-    assert (ofs + delta + size_chunk m = ofs + size_chunk m + delta) as EQ. ring.
-    rewrite EQ.
-    apply IHmc with (Mem0:=M) (gv:=gv); auto.
-    Case "wf_sb_mi".
-      split; auto.
-      SCase "Hnext1".
-        erewrite <- Mem.nextblock_store with (m1:=Mem0) in Hmap3; eauto.
-      SCase "Hnext2".
-        intros b1 b0 delta2 J.
-        apply Hmap4 in J.
-        apply Mem.nextblock_store in Hmstore.
-        rewrite Hmstore. auto.
-      SCase "mi_freeblocks0".
-        intros b0 J. apply mi_freeblocks0. intro J'. apply J.
-        eapply Mem.store_valid_block_1; eauto.
-      SCase "mi_mappedblocks0".
-        intros b0 b' delta0 J.
-        eapply Mem.store_valid_block_1; eauto.
-      SCase "mi_bounds".
-        intros b0 b' delta0 J.
-        apply mi_bounds0 in J.
-        apply Mem.bounds_store with (b':=b0) in Hmstore0; auto.
-        rewrite Hmstore0. rewrite J.
-        erewrite Mem.bounds_store with (m2:=Mem2'); eauto.
+  Transparent Mem.load.
+  unfold Mem.load in *. des_ifs. red.
+  eapply has_chunk__has_chunkb.
+  eapply decode_val_chunk; eauto. 
 Qed.
 
 Lemma simulation_mload_aux : forall Mem0 Mem2 b b2 delta mi mgb
@@ -1387,6 +867,8 @@ Proof.
     assert (ofs + delta + size_chunk a = ofs + size_chunk a + delta) as EQ. ring.
     rewrite EQ.
     rewrite Hmloads. eauto.
+    { esplits; eauto. chunk_auto.
+      eapply load_implies_has_chunkb; eauto. }
 Qed.
 
 Lemma simulation__fit_gv : forall maxb mi TD t Mem Mem2 gv1 gv1' gv2,
