src/Vellvm/memory_sim.v
@@ -69,12 +69,6 @@ Proof.
   destruct m, v; try inv Hchk; auto.
 Qed.
 
-Lemma val_inject__has_chunkb: forall mi v1 v2 m
-  (H : val_inject mi v1 v2),
-  Val.has_chunkb v1 m = Val.has_chunkb v2 m.
-Admitted.
-(* Proof. intros. inv H; auto. Qed. *)
-
 (** Monotone evolution of a memory injection. *)
 
 Definition inject_incr (f1 f2: meminj) : Prop :=
@@ -144,6 +138,17 @@ Proof.
   induction n; simpl; constructor; auto. constructor.
 Qed.  
 
+Lemma repeat_Undef_inject:
+  forall f n xs,
+    length xs = n ->
+    list_forall2 (memval_inject f) (list_repeat n Undef) xs.
+Proof.
+  ii.
+  ginduction n; ii; ss.
+  - destruct xs; ss. econs; eauto.
+  - destruct xs; ss. econs; eauto. econs; eauto.
+Qed.  
+
 (* Properties of proj_bytes. *)
 Lemma proj_bytes_inject_some:
   forall f vl vl',
@@ -162,22 +167,6 @@ Proof.
     inv H. rewrite (IHlist_forall2 l); auto.
     congruence.      
 Qed.
-
-Lemma proj_bytes_inject_none:
-  forall f vl vl',
-  list_forall2 (memval_inject f) vl vl' ->
-  proj_bytes vl = None ->
-  proj_bytes vl' = None.
-Proof.
-  (* induction 1; simpl. congruence. *)
-  (* inv H; try congruence. *)
-
-  (* intros. *)
-  (* remember (proj_bytes al) as R. *)
-  (* destruct R. *)
-  (*   inv H. rewrite (IHlist_forall2); auto. *)
-  (* Qed. *)
-Admitted.
 
 (* Properties of proj_pointer *)
 Definition meminj_no_overlap (f: meminj) : Prop :=
@@ -360,75 +349,75 @@ Proof.
 (* Qed. *)
 Admitted.
 
+Lemma memval_inject_implies
+      f vl1 vl2
+      (INJ: list_forall2 (Memdata.memval_inject f) vl1 vl2)
+  :
+    <<INJ: list_forall2 (memval_inject f) vl1 vl2>>
+.
+Proof.
+  red.
+  ginduction INJ; ii; ss.
+  { econs; eauto. }
+  econs; eauto.
+  inv H; try (by econs; eauto).
+Abort.
+
+Lemma memval_inject_implies
+      f v1 v2
+      (INJ: (memval_inject f) v1 v2)
+  :
+    <<INJ: (Memdata.memval_inject f) v1 v2>>
+.
+Proof.
+  red.
+  inv INJ; try (by econs; eauto).
+Qed.
+
+Lemma memval_inject_list_implies
+      f vl1 vl2
+      (INJ: list_forall2 (memval_inject f) vl1 vl2)
+  :
+    <<INJ: list_forall2 (Memdata.memval_inject f) vl1 vl2>>
+.
+Proof.
+  red.
+  ginduction INJ; ii; ss.
+  { econs; eauto. }
+  econs; eauto.
+  apply memval_inject_implies; eauto.
+Qed.
+
 (* Properties of encode/decode val *)
 Theorem encode_val_inject:
   forall f v1 v2 chunk,
   val_inject f v1 v2 ->
   list_forall2 (memval_inject f) (encode_val chunk v1) (encode_val chunk v2).
 Proof.
-(*   intros. inv H; simpl. *)
-(*     destruct chunk; solve [ *)
-(*       apply inj_bytes_inject | *)
-(*       apply repeat_Undef_inject_self | *)
-(*       apply repeat_Undef_inject_self]. *)
-(*     destruct chunk; solve [ *)
-(*       apply inj_bytes_inject | *)
-(*       apply repeat_Undef_inject_self | *)
-(*       apply repeat_Undef_inject_self]. *)
-(*     destruct chunk; solve [ *)
-(*       apply inj_bytes_inject | *)
-(*       apply repeat_Undef_inject_self | *)
-(*       apply repeat_Undef_inject_self]. *)
+  intros. inv H; simpl.
+    destruct chunk; solve [
+      apply inj_bytes_inject |
+      apply repeat_Undef_inject_self |
+      apply repeat_Undef_inject_self].
+    destruct chunk; solve [
+      apply inj_bytes_inject |
+      apply repeat_Undef_inject_self |
+      apply repeat_Undef_inject_self].
+    destruct chunk; solve [
+      apply inj_bytes_inject |
+      apply repeat_Undef_inject_self |
+      apply repeat_Undef_inject_self].
 
-(*     destruct chunk; try apply repeat_Undef_inject_self. *)
-(*     destruct (eq_nat_dec _ _); subst; try apply repeat_Undef_inject_self. *)
-(*       simpl; repeat econstructor; auto. *)
+    destruct chunk; try apply repeat_Undef_inject_self.
+    destruct (eq_nat_dec _ _); subst; try apply repeat_Undef_inject_self.
+      simpl; repeat econstructor; auto.
 
-(*     destruct chunk; try apply repeat_Undef_inject_self. *)
-(*     destruct (eq_nat_dec _ _); subst; try apply repeat_Undef_inject_self. *)
-(*       unfold inj_value; simpl; repeat econstructor; auto. *)
+    destruct chunk; try apply repeat_Undef_inject_self.
+    destruct (eq_nat_dec _ _); subst; try apply repeat_Undef_inject_self.
+      unfold inj_value; simpl; repeat econstructor; auto.
 
-(*     destruct chunk; try apply repeat_Undef_inject_self. *)
-(* Qed. *)
-Admitted.
-
-Theorem decode_val_inject:
-  forall f vl1 vl2 chunk,
-  meminj_no_overlap f ->
-  meminj_zero_delta f ->
-  list_forall2 (memval_inject f) vl1 vl2 ->
-  val_inject f (decode_val chunk vl1) (decode_val chunk vl2).
-Proof.
-  intros f vl1 vl2 chunk JJ JJ2 H. unfold decode_val.
-  case_eq (proj_bytes vl1); intros.
-    exploit proj_bytes_inject_some; eauto. intros H1. rewrite H1.
-    destruct chunk; try constructor.
-
-    {
-      destruct (proj_bytes vl2) eqn:T; ss; cycle 1.
-      { des_ifs. ss.
-        exploit proj_value_inject; eauto. intro INJ; des. inv INJ; ss.
-        econs; eauto.
-      }
-      {
-        des_ifs. ss.
-        des_ifs; try (by econs; ss).
-        - admit.
-        - admit.
-        - admit.
-      }
-    }
-(*     exploit proj_bytes_inject_none; eauto. intros. rewrite H1. *)
-(*     destruct chunk; auto. *)
-(*     destruct (eq_nat_dec _ _); subst; auto. *)
-(*       assert (H2 := H). simpl. *)
-(*       apply proj_value_inject in H2; auto. *)
-(*       remember (proj_value Q32 vl1) as v1. *)
-(*       remember (proj_value Q32 vl2) as v2. *)
-(*       inversion H2; auto. *)
-(*       rewrite <- H5 in H2. rewrite <- H6 in H2. auto. *)
-(* Qed. *)
-Admitted.
+    { apply repeat_Undef_inject. rewrite encode_val_length. ss. }
+Qed.
 
 Notation "a # b" := (Maps.PMap.get b a) (at level 1).
 Notation "a ! b" := (Maps.ZMap.get b a) (at level 1).
@@ -493,45 +482,6 @@ Proof.
   apply IHn. red; intros; apply H1; omega. 
 Qed.
 
-Lemma memval_inject_implies
-      f vl1 vl2
-      (INJ: list_forall2 (Memdata.memval_inject f) vl1 vl2)
-  :
-    <<INJ: list_forall2 (memval_inject f) vl1 vl2>>
-.
-Proof.
-  red.
-  ginduction INJ; ii; ss.
-  { econs; eauto. }
-  econs; eauto.
-  inv H; try (by econs; eauto).
-Abort.
-
-Lemma memval_inject_implies
-      f v1 v2
-      (INJ: (memval_inject f) v1 v2)
-  :
-    <<INJ: (Memdata.memval_inject f) v1 v2>>
-.
-Proof.
-  red.
-  inv INJ; try (by econs; eauto).
-Qed.
-
-Lemma memval_inject_list_implies
-      f vl1 vl2
-      (INJ: list_forall2 (memval_inject f) vl1 vl2)
-  :
-    <<INJ: list_forall2 (Memdata.memval_inject f) vl1 vl2>>
-.
-Proof.
-  red.
-  ginduction INJ; ii; ss.
-  { econs; eauto. }
-  econs; eauto.
-  apply memval_inject_implies; eauto.
-Qed.
-
 Lemma proj_bytes_not_inject
       f vl vl'
       (INJ: list_forall2 (memval_inject f) vl vl')
@@ -549,7 +499,8 @@ Proof.
   - inv H.
 Qed.
 
-Theorem decode_val_inject_compcert:
+(* copied && modified from compcert *)
+Theorem decode_val_inject:
   forall f vl1 vl2 chunk,
   meminj_no_overlap f ->
   meminj_zero_delta f ->
@@ -576,16 +527,6 @@ Proof.
     Print Memdata.memval_inject.
     Print memval_inject.
   }
-  (* assert (A: forall q fn, *)
-  (*    val_inject f (Val.load_result chunk (proj_value q vl1)) *)
-  (*                 (match proj_bytes vl2 with *)
-  (*                  | Some bl => fn bl *)
-  (*                  | None => Val.load_result chunk (proj_value q vl2) *)
-  (*                  end)). *)
-  (* { intros. destruct (proj_bytes vl2) as [bl2|] eqn:PB2. *)
-  (*   rewrite proj_value_undef. destruct chunk; auto. eapply proj_bytes_not_inject; eauto. congruence. *)
-  (*   apply val_load_result_inject. apply proj_value_inject; auto. *)
-  (* } *)
   des_ifs; ss.
 Qed.
 
